src/core/DY.Core.Attacker.Knowledge.Kleene.fst
@@ -1,0 +1,149 @@
+module DY.Core.Attacker.Knowledge.Kleene
+
+#set-options "--fuel 1 --ifuel 0"
+
+/// This module formalizes Kleene's fixpoint theorem
+/// https://en.wikipedia.org/wiki/Kleene_fixed-point_theorem
+
+type set_t (a:Type) = a -> prop
+
+val is_subset:
+  #a:Type ->
+  set_t a -> set_t a ->
+  prop
+let is_subset #a set1 set2 =
+  forall x. set1 x ==> set2 x
+
+noeq
+type directed_chain_t (a:Type) = {
+  sets: nat -> set_t a;
+  sets_monotonic:
+    i:nat -> j:nat ->
+    Lemma
+    (requires i <= j)
+    (ensures is_subset (sets i) (sets j))
+  ;
+}
+
+val union_set:
+  #a:Type ->
+  (nat -> set_t a) ->
+  set_t a
+let union_set #a sets =
+  fun x ->
+    exists n. sets n x
+
+val map_sets:
+  #a:Type ->
+  (set_t a -> set_t a) ->
+  (nat -> set_t a) ->
+  (nat -> set_t a)
+let map_sets #a f sets =
+  fun n -> fun x ->
+    f (sets n) x
+
+noeq
+type f_properties (#a:Type) (f:set_t a -> set_t a) = {
+  is_scott_continuous:
+    chain:directed_chain_t a -> x:a ->
+    Lemma (f (union_set chain.sets) x <==> union_set (map_sets f chain.sets) x)
+  ;
+  // scott continuity implies monotonicity,
+  // but proving so requires extensionality on sets,
+  // so instead we ask the user to prove it manually
+  is_monotonic:
+    set1:set_t a -> set2:set_t a ->
+    Lemma
+    (requires is_subset set1 set2)
+    (ensures is_subset (f set1) (f set2))
+  ;
+}
+
+val mk_weakest_fixpoint_aux:
+  #a:Type ->
+  (set_t a -> set_t a) -> nat ->
+  set_t a
+let rec mk_weakest_fixpoint_aux #a f n =
+  fun x ->
+    if n = 0 then (
+      False
+    ) else (
+      f (mk_weakest_fixpoint_aux f (n-1)) x
+    )
+
+val mk_weakest_fixpoint:
+  #a:Type ->
+  (set_t a -> set_t a) ->
+  set_t a
+let mk_weakest_fixpoint #a f =
+  union_set (mk_weakest_fixpoint_aux f)
+
+val mk_weakest_fixpoint_aux_is_monotonic_consecutive:
+  #a:Type ->
+  f:(set_t a -> set_t a) -> f_properties f ->
+  i:nat ->
+  Lemma (is_subset (mk_weakest_fixpoint_aux f i) (mk_weakest_fixpoint_aux f (i+1)))
+let rec mk_weakest_fixpoint_aux_is_monotonic_consecutive #a f f_props i =
+  if i = 0 then ()
+  else (
+    mk_weakest_fixpoint_aux_is_monotonic_consecutive f f_props (i-1);
+    f_props.is_monotonic (mk_weakest_fixpoint_aux f (i-1)) (mk_weakest_fixpoint_aux f i)
+  )
+
+val mk_weakest_fixpoint_aux_is_monotonic:
+  #a:Type ->
+  f:(set_t a -> set_t a) -> f_properties f ->
+  i:nat -> j:nat ->
+  Lemma
+  (requires i <= j)
+  (ensures is_subset (mk_weakest_fixpoint_aux f i) (mk_weakest_fixpoint_aux f j))
+let rec mk_weakest_fixpoint_aux_is_monotonic #a f f_properties i j =
+  if i = j then ()
+  else (
+    mk_weakest_fixpoint_aux_is_monotonic f f_properties i (j-1);
+    mk_weakest_fixpoint_aux_is_monotonic_consecutive f f_properties (j-1)
+  )
+
+val mk_weakest_fixpoint_is_fixpoint:
+  #a:Type ->
+  f:(set_t a -> set_t a) ->
+  f_properties f ->
+  Lemma
+  (is_subset (f (mk_weakest_fixpoint f)) (mk_weakest_fixpoint f))
+let mk_weakest_fixpoint_is_fixpoint #a f f_props =
+  introduce forall x. f (mk_weakest_fixpoint f) x ==> mk_weakest_fixpoint f x
+  with introduce _ ==> _ with _. (
+    assert(f (mk_weakest_fixpoint f) x);
+    assert(f (union_set (mk_weakest_fixpoint_aux f)) x);
+    f_props.is_scott_continuous {
+      sets = mk_weakest_fixpoint_aux f;
+      sets_monotonic = mk_weakest_fixpoint_aux_is_monotonic f f_props;
+    } x;
+    assert(forall n. f (mk_weakest_fixpoint_aux f n) x ==> mk_weakest_fixpoint_aux f (n+1) x);
+    assert(mk_weakest_fixpoint f x)
+  )
+
+val mk_weakest_fixpoint_is_weakest_aux:
+  #a:Type ->
+  f:(set_t a -> set_t a) -> f_properties f ->
+  set:set_t a ->
+  n:nat ->
+  Lemma
+  (requires is_subset (f set) set)
+  (ensures is_subset (mk_weakest_fixpoint_aux f n) set)
+let rec mk_weakest_fixpoint_is_weakest_aux #a f f_props set n =
+  if n = 0 then ()
+  else (
+    mk_weakest_fixpoint_is_weakest_aux f f_props set (n-1);
+    f_props.is_monotonic (mk_weakest_fixpoint_aux f (n-1)) set
+  )
+
+val mk_weakest_fixpoint_is_weakest:
+  #a:Type ->
+  f:(set_t a -> set_t a) -> f_properties f ->
+  set:set_t a ->
+  Lemma
+  (requires is_subset (f set) set)
+  (ensures is_subset (mk_weakest_fixpoint f) set)
+let mk_weakest_fixpoint_is_weakest #a f f_props set =
+  FStar.Classical.forall_intro (FStar.Classical.move_requires (mk_weakest_fixpoint_is_weakest_aux f f_props set))
